$$\begin{align}
\text{Finding slope of the tangent line} \\
\lim_{ h \to 0 }= \frac{\frac{4}{x+h}-\frac{4}{x}}{h} \\
\text{Get a common base} \\
\lim_{ h \to 0 }= \frac{\frac{4(x)}{x(x+h)}-\frac{4(x+h)}{x(x+h)}}{h} \\
\text{Combine fractions} \\
\lim_{ h \to 0 }= \frac{\frac{4x-4(x+h)}{x(x+h)}}{h}  \\
\text{Expand} \\
\lim_{ h \to 0 }= \frac{\frac{4x-4x-4h}{x(x+h)}}{h} \\
\text{Simplify} \\
\lim_{ h \to 0 }= \frac{\frac{-4h}{x(x+h)}}{h}  \\
\text{Apply fraction rule} \frac{\frac{a}{b}}{c}=\frac{a}{b*c} \\
\lim_{ h \to 0 }= \frac{-4h}{(x(x+h))(h)} \\
\text{Simplify} \\
\lim_{ h \to 0 }= \frac{-4}{x(x+h)}  \\
\text{Take lim h approaching 0 to get tangent line} slope\\
\lim_{ h \to 0 }= \frac{-4}{x(x+0)} \\
\lim_{ h \to 0 }= \frac{-4}{x(x)} \\
\lim_{ h \to 0 }= \frac{-4}{x^2} \\
\text{Slope of tangent line (derivative) is} f'(x)=\frac{-4}{x^{2}}  \\
 \\
\text{Find slope (m) of tangent line at }x=6 \\
f'(x)=\frac{-4}{x^{2}} \\
f'(6)= \frac{-4}{36} \to \frac{-2}{18} \to \frac{-1}{9}  \\
\text{Find point of f(x) at x=6} \\
f(x)=\frac{4}{x} \\
f(6)=\frac{4}{6} \to \frac{2}{3} \\
\text{Find the equation of tangent line at }x=6 \text{ using point-slope formula} \\
y-y_{1}=m(x-x_{1}) \\
y-\frac{2}{3}=\frac{-1}{9}(x-6) \\
\text{Multiply through} \\
y-\frac{2}{3}=\frac{-1}{9}x+ \frac{6}{9} \\
\text{Move y1 over} \\
y=\frac{-1}{9}x+ \frac{6}{9} + \frac{-2}{3} \\
\text{Add fractions} \\
y=\frac{-1}{9}x+ \frac{2}{3} + \frac{2}{3}  \\
y=\frac{-1}{9}x + \frac{4}{3} 
\end{align}$$




$$lim_{x\to+\infty} \frac{3p\sqrt{4h^{2}+x^{2}}+x}{xh}=\frac{3p+1}{h}$$
$$ $$$$\begin{align}
lim_{x\to+\infty} \frac{3p\sqrt{4h^{2}+x^{2}}+x}{xh} \\
lim_{x\to+\infty} =\frac{3p+1}{h} \\
lim_{x\to+\infty} =\frac{3p}{h}+ \frac{1}{h}
\end{align}$$

$$\left(d\right)=\frac{\left(\left(p\right)\left(\pi\right)\left(r\right)\left(\sqrt{h^{2}+r^{2}}\right)+\pi\left(r^{2}\right)\right)}{\left(\frac{1}{3}\right)\left(\pi\right)\left(r^{2}\right)\left(h\right)}\ \to\ \left(d\right)=\frac{3p\sqrt{r^{2}+h^{2}}+r}{r\left(h\right)}$$


$$\lim_{ x \to \infty } \frac{3p \sqrt{ r^{2}+h^{2 }})+ r}{(r)(h)}=0$$$$\lim_{h\to\infty}\frac{3p\sqrt{x^{2}+h^{2}}+x}{(x)(h)}=\frac{3p}{x}$$

$$\left(d\right)=\frac{\left(\left(p\right)\left(\pi\right)\left(r\right)\left(\sqrt{h^{2}+r^{2}}\right)+\pi\left(r^{2}\right)\right)}{\left(\frac{1}{3}\right)\left(\pi\right)\left(r^{2}\right)\left(h\right)}\ \to\ \left(d\right)=\frac{3p\sqrt{r^{2}+h^{2}}+r)}{(r)\left(h\right)}$$

$$\left(d\right)=\frac{\left(p\right)(3x^{2}\sqrt{25+10\sqrt{5}})}{\frac{15+7\sqrt{5}}{4}x^{3}}\ \to\ \left(d\right)=-\frac{3\left(15-7\sqrt{5}\right)(\sqrt{25+10\sqrt{5}})(p)}{5x}$$
